Veir/OpCode.lean
@@ -25,6 +25,7 @@ public import Veir.Dialects.HW.OpInfo
 public import Veir.Dialects.Verif.OpInfo
 public import Veir.Dialects.PDL.OpInfo
 public import Veir.Dialects.Test.OpInfo
+public import Veir.Dialects.LLZK.Felt.OpInfo
 
 open Std
 
